SSA/Experimental/Bits/Fast/Circuit.lean
@@ -13,8 +13,7 @@ to the arity of `α`. See also `eval` for the explicit conversion of a circuit t
 inductive Circuit (α : Type u) : Type u
   | tru : Circuit α
   | fals : Circuit α
-  /-- `var b x` represents literal `x` or the negated literat `¬x`,
-      depending on the value of `b` -/
+  /-- `var b x` represents literal `x` if `b = true` or the negated literat `¬x` if `b = false` -/
   | var : Bool → α → Circuit α
   | and : Circuit α → Circuit α → Circuit α
   | or : Circuit α → Circuit α → Circuit α
@@ -22,6 +21,7 @@ inductive Circuit (α : Type u) : Type u
 deriving Repr
 
 namespace Circuit
+
 variable {α : Type u} {β : Type v}
 
 def vars [DecidableEq α] : Circuit α → List α
@@ -759,5 +759,9 @@ lemma always_true_iff [DecidableEq α] (c : Circuit α) :
 instance [DecidableEq α] : DecidableRel ((· ≤· ) : Circuit α → Circuit α → Prop) :=
   λ c₁ c₂ => decidable_of_iff (always_true ((~~~ c₁).or c₂)) <|
     by simp [always_true_iff, le_def, or_iff_not_imp_left]
+
+/-- Negate the value of the circuit -/
+def not {α : Type u} (c : Circuit α) : Circuit α := 
+  .xor .tru c
 
 end Circuit
