SSA/Experimental/Bits/Fast/Defs.lean
@@ -40,13 +40,10 @@ inductive Term : Type
 | incr : Term → Term
 /-- Decrement (i.e., subtract one) -/
 | decr : Term → Term
-/-- `repeatBit` is an operation that will repeat the infinitely repeat the
-least significant `true` bit of the input.
-
-That is `repeatBit t` is all-zeroes iff `t` is all-zeroes.
-Otherwise, there is some number `k` s.t. `repeatBit t` is all-ones after
-dropping the least significant `k` bits  -/
-| repeatBit : Term → Term
+-- | shiftL : Term → Nat → Term : shift left by `k` bits.
+-- | lshiftR : Term → Nat → Term : logical shift right by `k` bits.
+-- bollu: I don't think we can do ashiftr, because it's output is 'irregular',
+--   hence, I don't anticipate us implementing it.
 
 open Term
 
@@ -58,9 +55,9 @@ given a value for the free variables in `t`.
 Note that we don't keep track of how many free variable occur in `t`,
 so eval requires us to give a value for each possible variable.
 -/
-def Term.eval (t : Term) (vars : Nat → BitStream) : BitStream :=
+def Term.eval (t : Term) (vars : List BitStream) : BitStream :=
   match t with
-  | var n       => vars n
+  | var n       => vars[n]!
   | zero        => BitStream.zero
   | one         => BitStream.one
   | negOne      => BitStream.negOne
@@ -74,7 +71,7 @@ def Term.eval (t : Term) (vars : Nat → BitStream) : BitStream :=
   | neg t       => -(Term.eval t vars)
   | incr t      => BitStream.incr (Term.eval t vars)
   | decr t      => BitStream.decr (Term.eval t vars)
-  | repeatBit t => BitStream.repeatBit (Term.eval t vars)
+ -- | repeatBit t => BitStream.repeatBit (Term.eval t vars)
 
 instance : Add Term := ⟨add⟩
 instance : Sub Term := ⟨sub⟩
@@ -102,7 +99,7 @@ a term like `var 10` only has a single free variable, but its arity will be `11`
 | neg t => arity t
 | incr t => arity t
 | decr t => arity t
-| repeatBit t => arity t
+-- | repeatBit t => arity t
 
 /--
 Evaluate a term `t` to the BitStream it represents.
@@ -142,4 +139,183 @@ and only require that many bitstream values to be given in `vars`.
   | neg t       => -(Term.evalFin t vars)
   | incr t      => BitStream.incr (Term.evalFin t vars)
   | decr t      => BitStream.decr (Term.evalFin t vars)
-  | repeatBit t => BitStream.repeatBit (Term.evalFin t vars)
+  -- | repeatBit t => BitStream.repeatBit (Term.evalFin t vars)
+
+
+/--
+The fragment of predicate logic that we support in `bv_automata`.
+Currently, we support equality, conjunction, disjunction, and negation.
+This can be expanded to also support arithmetic constraints such as unsigned-less-than.
+
+Meaning of the denotation:
+
+`p w = false` iff the predicate holds *at* width w
+-/
+-- a < b <=> a - b < 0
+-- a <= 0 <=> a < 0 ∨ a = 0
+-- a > b <=> b < a <=> b - a < 0
+inductive Predicate : Type where
+| eq (t₁ t₂ : Term) : Predicate
+| neq (t₁ t₂ : Term) : Predicate
+| ult (t₁ t₂ : Term) : Predicate
+| ule (t₁ t₂ : Term) : Predicate
+| slt (t₁ t₂ : Term) : Predicate
+| sle (t₁ t₂ : Term) : Predicate
+| land  (p q : Predicate) : Predicate
+| lor (p q : Predicate) : Predicate
+
+
+
+/--
+If they are equal so far, then `t1 ^^^ t2`.scanOr will be 0.
+-/
+def Predicate.evalEq (t₁ t₂ : BitStream) : BitStream := (t₁ ^^^ t₂).scanOr
+/--
+If they have been equal so far, then `BitStream.nxor t₁ t₂`.scanAnd will be 1.
+Start by assuming that they are not (not equal) i.e. that they are equal, and the 
+   initial value of the preciate is false / `1`.
+If their values ever differ, then we know that we will have `a[i] == b[i]` to be `false`.
+From this point onward, they will always disagree, and thus the predicate should become `0`.
+-/
+-- def Predicate.evalNeq (t₁ t₂ : BitStream) : BitStream := (BitStream.nxor t₁ t₂).scanAnd
+def Predicate.evalNeq (t₁ t₂ : BitStream) : BitStream := 
+  let bs : BitStream := fun i => if t₁ i != t₂ i then false else true
+  bs.scanAnd
+
+/-
+If they have been `0` so far, then `t1 &&& t2 |>.scanOr` will be `1`.
+-/
+def Predicate.evalLor (t₁ t₂ : BitStream) : BitStream := (t₁ &&& t₂)
+
+-- | And does not seem to work?
+def Predicate.evalLand (t₁ t₂ : BitStream) : BitStream := (t₁ ||| t₂)
+
+
+/-- 
+Evaluate whether 't₁ <ᵤ t₂'.
+This is defined by computing the borrow bit of 't₁ - t₂'.
+If the borrow bit is `1`, then we know that `t₁ < t₂', so we return a `0`.
+Otherwise, we know that 't₁ ≥ t₂'.
+-/
+def Predicate.evalUlt (t₁ t₂ : BitStream) : BitStream := ~~~ (t₁.borrow t₂)
+
+/-- 
+Evaluate whether 't₁ <s t₂'.
+This is defined by computing the most significant bit of 't₁ - t₂'.
+IF the `msb is 1`, then `t₁ - t₂ <s 0`, and thus `t₁ <s t₂'.
+-/
+def Predicate.evalSlt (t₁ t₂ : BitStream) : BitStream := ~~~ (t₁ - t₂)
+
+-- | leq (t₁ t₂ : Term) : Predicate -> simulate in terms of lt and eq
+open BitStream in
+/--
+Evaluate a term predicate `p` to the BitStream it represents,
+where the predicate is `true` at index `i` if and only if the predicate,
+when truncated to index `i`, is true.
+-/
+def Predicate.eval (p : Predicate) (vars : List BitStream) : BitStream :=
+  match p with
+  | eq t₁ t₂ => Predicate.evalEq (t₁.eval vars) (t₂.eval vars)
+  /-
+  If it is ever not equal, then we want to stay not equals for ever.
+  So, if the 'a = b' returns 'false' at some index 'i', we will stay false
+  for all indexes '≥ i'.
+  -/
+  | neq t1 t2 => Predicate.evalNeq (t1.eval vars) (t2.eval vars)
+  | lor p q => Predicate.evalLor (p.eval vars) (q.eval vars)
+  | land p q => Predicate.evalLand (p.eval vars) (q.eval vars)
+  | ult t₁ t₂ => Predicate.evalUlt (t₁.eval vars) (t₂.eval vars)
+  | ule t₁ t₂ => 
+     Predicate.evalLor 
+       (Predicate.evalEq (t₁.eval vars) (t₂.eval vars))
+       (Predicate.evalUlt (t₁.eval vars) (t₂.eval vars))
+  | slt t₁ t₂ => Predicate.evalSlt (t₁.eval vars) (t₂.eval vars)
+  | sle t₁ t₂ => Predicate.evalLor 
+       (Predicate.evalEq (t₁.eval vars) (t₂.eval vars))
+       (Predicate.evalSlt (t₁.eval vars) (t₂.eval vars))
+
+@[simp]
+theorem Bool.xor_false_iff_eq : ∀ (a b : Bool), (a ^^ b) = false ↔ a = b := by decide
+
+section Predicate
+/-- If something is always true, then it is eventually always true. -/
+theorem eventually_all_zeroes_of_all_zeroes (b : BitStream) (h : ∀ n, b n = false) : ∃ (N : Nat), ∀ n ≥ N, b n = false := by
+  exists Nat.zero
+  simp [h]
+
+
+/-- If the scanOr of something is eventually always zeroes, then it must be all zeroes. -/
+theorem all_zeroes_of_scanOr_eventually_all_zeroes (b : BitStream) (h : ∃ (N : Nat), ∀ n ≥ N, b.scanOr n = false) : ∀ n, b n = false := by
+  intros n
+  have ⟨N, h⟩ := h
+  simp [BitStream.scanOr_false_iff] at h
+  apply h (n := max N n) <;> omega
+
+end Predicate
+
+@[simp] def Predicate.arity : Predicate → Nat
+| .eq t1 t2 => max t1.arity t2.arity
+| .lor p q => max p.arity q.arity
+| .land p q => max p.arity q.arity
+| .neq t₁ t₂ => max t₁.arity t₂.arity
+| .ult t₁ t₂ => max t₁.arity t₂.arity
+| .ule t₁ t₂ => max (max t₁.arity t₂.arity) (max t₁.arity t₂.arity)
+| .slt t₁ t₂ => max t₁.arity t₂.arity
+| .sle t₁ t₂ => max (max t₁.arity t₂.arity) (max t₁.arity t₂.arity)
+
+@[simp]
+def Predicate.evalFinLor (x₁ x₂ : BitStream) : BitStream := 
+    (x₁ &&& x₂)
+
+@[simp]
+def Predicate.evalFinEq (x₁ x₂ : BitStream) : BitStream := 
+    (x₁ ^^^ x₂)
+
+@[simp]
+def Predicate.evalFinSlt (x₁ x₂ : BitStream) : BitStream := 
+  ~~~ (x₁ - x₂)
+
+@[simp]
+def Predicate.evalFinUlt (x₁ x₂ : BitStream) : BitStream := 
+  ~~~ (x₁.borrow x₂)
+
+/-- Denote a predicate into a bitstream, where the ith bit tells us if it is true in the ith state -/
+@[simp] def Predicate.evalFin (p : Predicate) (vars : Fin (arity p) → BitStream) : BitStream :=
+match p with
+| .eq t₁ t₂ =>
+    let x₁ := t₁.evalFin (fun i => vars (Fin.castLE (by simp [arity]) i))
+    let x₂ := t₂.evalFin (fun i => vars (Fin.castLE (by simp [arity]) i))
+    Predicate.evalFinEq x₁ x₂
+| .neq t₁ t₂  =>
+    let x₁ := t₁.evalFin (fun i => vars (Fin.castLE (by simp [arity]) i))
+    let x₂ := t₂.evalFin (fun i => vars (Fin.castLE (by simp [arity]) i))
+    (x₁.nxor x₂)
+| .land p q =>
+  -- if both `p` and `q` are logically true (i.e. the predicate is `false`),
+  -- only then should we return a `false`.
+  let x₁ := p.evalFin (fun i => vars (Fin.castLE (by simp [arity]) i))
+  let x₂ := q.evalFin (fun i => vars (Fin.castLE (by simp [arity]) i))
+  (x₁ ||| x₂)
+| .lor p q =>
+  -- If either of the predicates are `false`, then result is `false`.
+  let x₁ := p.evalFin (fun i => vars (Fin.castLE (by simp [arity]) i))
+  let x₂ := q.evalFin (fun i => vars (Fin.castLE (by simp [arity]) i))
+  Predicate.evalFinLor x₁ x₂
+| .slt p q => 
+  let x₁ := p.evalFin (fun i => vars (Fin.castLE (by simp [arity]) i))
+  let x₂ := q.evalFin (fun i => vars (Fin.castLE (by simp [arity]) i))
+  Predicate.evalFinSlt x₁ x₂
+| .sle p q => 
+  let x₁ := p.evalFin (fun i => vars (Fin.castLE (by simp [arity]) i))
+  let x₂ := q.evalFin (fun i => vars (Fin.castLE (by simp [arity]) i))
+  Predicate.evalFinLor (Predicate.evalFinSlt x₁ x₂) (Predicate.evalFinEq x₁ x₂)
+| .ult p q => 
+  let x₁ := p.evalFin (fun i => vars (Fin.castLE (by simp [arity]) i))
+  let x₂ := q.evalFin (fun i => vars (Fin.castLE (by simp [arity]) i))
+  (Predicate.evalFinUlt x₁ x₂)
+| .ule p q => 
+  let x₁ := p.evalFin (fun i => vars (Fin.castLE (by simp [arity]) i))
+  let x₂ := q.evalFin (fun i => vars (Fin.castLE (by simp [arity]) i))
+  Predicate.evalFinLor (Predicate.evalFinUlt x₁ x₂) (Predicate.evalFinEq x₁ x₂)
+
+
