SSA/Experimental/Bits/Fast/Reflect.lean
@@ -1,0 +1,817 @@
+/-
+Released under Apache 2.0 license as described in the file LICENSE.
+
+
+This file reflects the semantics of bitstreams, terms, predicates, and FSMs
+into lean bitvectors.
+
+We use `grind_norm` to convert the expression into negation normal form.
+
+Authors: Siddharth Bhat
+-/
+import Mathlib.Data.Bool.Basic
+import Mathlib.Data.Fin.Basic
+import SSA.Experimental.Bits.Fast.BitStream
+import SSA.Experimental.Bits.Fast.Defs
+import SSA.Experimental.Bits.Fast.FiniteStateMachine
+import SSA.Experimental.Bits.Fast.Attr
+import SSA.Experimental.Bits.Fast.Decide
+import Lean.Meta.ForEachExpr
+import Lean.Meta.Tactic.Simp.BuiltinSimprocs.BitVec
+
+import Lean
+
+/--
+Denote a bitstream into the underlying bitvector.
+-/
+def BitStream.denote (s : BitStream) (w : Nat) : BitVec w := s.toBitVec w
+
+@[simp] theorem BitStream.denote_zero : BitStream.denote BitStream.zero w = 0#w := by
+  simp [denote, toBitVec]
+  sorry
+
+@[simp] theorem BitStream.denote_negOne : BitStream.denote BitStream.negOne w = BitVec.allOnes w := by
+  simp [denote, toBitVec]
+  sorry
+
+
+/-- Denote a Term into its underlying bitvector -/
+def Term.denote (w : Nat) (t : Term) (vars : List (BitVec w)) : BitVec w :=
+  match t with
+  | var n => vars[n]!
+  | zero => 0#w
+  | negOne => BitVec.allOnes w
+  | one  => 1#w
+  | and a b => (a.denote w vars) &&& (b.denote w vars)
+  | or a b => (a.denote w vars) ||| (b.denote w vars)
+  | xor a b => (a.denote w vars) ^^^ (b.denote w vars)
+  | not a => ~~~ (a.denote w vars)
+  | add a b => (a.denote w vars) + (b.denote w vars)
+  | sub a b => (a.denote w vars) - (b.denote w vars)
+  | neg a => - (a.denote w vars)
+  | incr a => (a.denote w vars) + 1#w
+  | decr a => (a.denote w vars) - 1#w
+  | ls bit a => (a.denote w vars).shiftConcat bit
+
+theorem Term.eval_eq_denote (t : Term) (w : Nat) (vars : List (BitVec w)) :
+    (t.eval (vars.map BitStream.ofBitVec)).denote w = t.denote w vars := by
+  induction t generalizing w vars
+  repeat sorry
+
+def Predicate.denote (p : Predicate) (w : Nat) (vars : List (BitVec w)) : Prop :=
+  match p with
+  | .eq t₁ t₂ => t₁.denote w vars = t₂.denote w vars
+  | .neq t₁ t₂ => t₁.denote w vars ≠ t₂.denote w vars
+  | .land  p q => p.denote w vars ∧ q.denote w vars
+  | .lor  p q => p.denote w vars ∨ q.denote w vars
+  | .sle  t₁ t₂ => (((t₁.denote w vars).sle (t₂.denote w vars)) = true)
+  | .slt  t₁ t₂ => ((t₁.denote w vars).slt (t₂.denote w vars)) = true
+  | .ule  t₁ t₂ => ((t₁.denote w vars) ≤ (t₂.denote w vars))
+  | .ult  t₁ t₂ => (t₁.denote w vars) < (t₂.denote w vars)
+
+/--
+The semantics of a predicate:
+The predicate, when evaluated, at index `i` is false iff the denotation is true.
+-/
+theorem Predicate.eval_eq_denote (w : Nat) (p : Predicate) (vars : List (BitVec w)) :
+    (p.eval (vars.map BitStream.ofBitVec) w = false) ↔ p.denote w vars := by
+  induction p generalizing vars w
+  repeat sorry
+
+
+/-- To prove that `p` holds, it suffices to show that `p.eval ... = false`. -/
+theorem Predicate.denote_of_eval_eq {p : Predicate}
+    (heval : ∀ (w : Nat) (vars : List BitStream), p.eval vars w = false) : 
+    ∀ (w : Nat) (vars : List (BitVec w)), p.denote w vars := by
+  intros w vars
+  apply p.eval_eq_denote w vars |>.mp (heval w <| vars.map BitStream.ofBitVec)
+
+
+def Reflect.Map.empty : List (BitVec w) := []
+
+def Reflect.Map.append (w : Nat) (s : BitVec w)  (m : List (BitVec w)) : List (BitVec w) := m.append [s]
+
+def Reflect.Map.get (ix : ℕ) (s : BitVec w)  (m : List (BitVec w)) : BitVec w := m[ix]!
+
+
+namespace NNF
+open Lean Elab Meta
+
+/-- convert goal to negation normal form, by running appropriate lemmas from `grind_norm`, and reverting all hypothese. -/
+def runNNFSimpSet (g : MVarId) : MetaM (Option MVarId) := do
+  let some ext ← (getSimpExtension? `grind_norm)
+    | throwError m!"[bv_nnf] Error: 'grind_norm' simp attribute not found!"
+  let theorems ← ext.getTheorems
+  let theorems ←  theorems.erase (Origin.decl ``ne_eq)
+  let some ext ← (Simp.getSimprocExtension? `grind_norm)
+    | throwError m!"[bv_nnf] Error: 'grind_norm' simp attribute not found!"
+  let simprocs ← ext.getSimprocs
+  let config : Simp.Config := { Simp.neutralConfig with
+    failIfUnchanged   := false,
+  }
+  let ctx ← Simp.mkContext (config := config)
+    (simpTheorems := #[theorems])
+    (congrTheorems := ← Meta.getSimpCongrTheorems)
+  match ← simpGoal g ctx (simprocs := #[simprocs]) with
+  | (none, _) => return none
+  | (some (_newHyps, g'), _) => pure g'
+
+open Lean Elab Meta Tactic in
+/-- Convert the goal into negation normal form. -/
+elab "bv_nnf" : tactic => do
+  liftMetaTactic fun g => do
+    match ← runNNFSimpSet g with
+    | none => return []
+    | some g => do
+      -- revert after running the simp-set, so that we don't transform
+      -- with `forall_and : (∀ x, p x ∧ q x) ↔ (∀ x, p x) ∧ (∀ x, q x)`.
+      -- TODO(@bollu): This opens up an interesting possibility, where we can handle smaller problems
+      -- by just working on disjunctions.
+      -- let g ← g.revertAll
+      return [g]
+
+attribute [grind_norm] BitVec.not_lt
+attribute [grind_norm] BitVec.not_le
+
+@[grind_norm]
+theorem sle_iff_slt_eq_false {a b : BitVec w} : a.slt b = false ↔ b.sle a := by
+  constructor <;>
+  intros h <;>
+  simp [BitVec.sle, BitVec.slt] at h ⊢ <;>
+  omega
+
+@[grind_norm]
+theorem slt_iff_sle_eq_false {a b : BitVec w} : a.sle b = false ↔ b.slt a := by
+  constructor <;>
+  intros h <;>
+  simp [BitVec.sle, BitVec.slt] at h ⊢ <;>
+  omega
+--  ne_eq: (a ≠ b) = ¬(a = b) := rfl
+attribute [- grind_norm] ne_eq -- TODO(bollu): Debate with grind maintainer about having `a ≠ b → ¬ (a = b)` in the simp-set?
+@[grind_norm] theorem not_eq_iff_neq : (¬ (a = b)) = (a ≠ b) := by rfl
+
+/--
+warning: 'ne_eq' does not have [simp] attribute
+---
+warning: declaration uses 'sorry'
+---
+info: w : ℕ
+⊢ (∀ (x x_1 : BitVec w), x_1 ≤ x) ∧ ∀ (x x_1 : BitVec w), x ≤ x_1 ∨ x_1 < x ∨ x ≤ x_1 ∨ x ≠ x_1
+-/
+#guard_msgs in example : ∀ (a b : BitVec w),  ¬ (a < b ∨ a > b ∧ a ≤ b ∧ a > b ∧ (¬ (a ≠ b))) := by
+ bv_nnf; trace_state; sorry
+
+/--
+warning: 'ne_eq' does not have [simp] attribute
+---
+warning: declaration uses 'sorry'
+---
+info: w : ℕ
+⊢ ∀ (a b : BitVec w), a &&& b ≠ 0#w ∨ a = b
+-/
+#guard_msgs in example : ∀ (a b : BitVec w), a &&& b = 0#w → a = b := by
+ bv_nnf; trace_state; sorry
+
+end NNF
+
+/-
+Armed with the above, we write a proof by reflection principle.
+This is adapted from Bits/Fast/Tactic.lean, but is cleaned up to build 'nice' looking environments
+for reflection, rather than ones based on hashing the 'fvar', which can also have weird corner cases due to hash collisions.
+
+TODO(@bollu): For now, we don't reflects constants properly, since we don't have arbitrary constants in the term language (`Term`).
+TODO(@bollu): We also assume that the goals are in negation normal form, and if we not, we bail out. We should make sure that we write a tactic called `nnf` that transforms goals to negation normal form.
+-/
+
+namespace Reflect
+open Lean Meta Elab Tactic
+
+/-- The free variables in the term that is reflected. -/
+structure ReflectMap where
+  /-- Map expressions to their index in the eventual `Reflect.Map`. -/
+  exprs : Std.HashMap Expr Nat
+
+
+instance : EmptyCollection ReflectMap where
+  emptyCollection := { exprs := ∅ }
+
+abbrev ReflectedExpr := Expr
+
+/--
+Insert expression 'e' into the reflection map. This returns the map,
+as well as the denoted term.
+-/
+def ReflectMap.findOrInsertExpr (m : ReflectMap) (e : Expr) : ReflectedExpr × ReflectMap :=
+  let (ix, m) := match m.exprs.get? e with
+    | some ix =>  (ix, m)
+    | none =>
+      let ix := m.exprs.size
+      (ix, { m with exprs := m.exprs.insert e ix })
+  let e :=  mkApp (mkConst ``Term.var) (mkNatLit ix)
+  (e, m)
+    
+
+/--
+Convert the meta-level `ReflectMap` into an object level `Reflect.Map` by
+repeatedly calling `Reflect.Map.empty` and `Reflect.Map.set`.
+-/
+def ReflectMap.toExpr (xs : ReflectMap) (w : Expr) : MetaM ReflectedExpr := do
+  let mut out := mkApp (mkConst ``Reflect.Map.empty) w
+  let exprs := xs.exprs.toArray.qsort (fun ei ej => ei.2 < ej.2)
+  for (e, _) in exprs do
+    -- The 'exprs' will be in order, with 0..n
+    /- Append the expressions into the array -/
+    out := mkAppN (mkConst ``Reflect.Map.append) #[w, e, out]
+  return out
+
+instance : ToMessageData ReflectMap where
+  toMessageData exprs := Id.run do
+    -- sort in order of index.
+    let es := exprs.exprs.toArray.qsort (fun a b => a.2 < b.2)
+    let mut lines := es.map (fun (e, i) => m!"{i}→{e}")
+    return m!"[" ++ m!" ".joinSep lines.toList ++ m!"]"
+/--
+Result of reflection, where we have a collection of bitvector variables,
+along with the bitwidth and the final term.
+-/
+structure ReflectResult where
+  /-- Map of 'free variables' in the bitvector expression,
+  which are indexed as Term.var. This array is used to build the environment for decide.
+  -/
+  bvToIxMap : ReflectMap
+  e : ReflectedExpr
+
+instance : ToMessageData ReflectResult where
+  toMessageData result := m!"{result.e} {result.bvToIxMap}"
+
+
+
+/--
+info: ∀ {w : Nat} (a b : BitVec w),
+  @Eq (BitVec w) (@HAdd.hAdd (BitVec w) (BitVec w) (BitVec w) (@instHAdd (BitVec w) (@BitVec.instAdd w)) a b)
+    (BitVec.ofNat w (@OfNat.ofNat Nat 0 (instOfNatNat 0))) : Prop
+-/
+#guard_msgs in set_option pp.explicit true in
+#check ∀ {w : Nat} (a b: BitVec w), a + b = 0#w
+
+/--
+info: ∀ {w : Nat} (a : BitVec w),
+  @Eq (BitVec w) (@Neg.neg (BitVec w) (@BitVec.instNeg w) a)
+    (BitVec.ofNat w (@OfNat.ofNat Nat 0 (instOfNatNat 0))) : Prop
+-/
+#guard_msgs in set_option pp.explicit true in
+#check ∀ {w : Nat} (a : BitVec w), - a = 0#w
+
+
+/--
+info: ∀ {w : Nat} (a : BitVec w),
+  @LT.lt (BitVec w) (@instLTBitVec w) a (BitVec.ofNat w (@OfNat.ofNat Nat 0 (instOfNatNat 0))) : Prop
+-/
+#guard_msgs in set_option pp.explicit true in
+#check ∀ {w : Nat} (a : BitVec w),  a  < 0#w
+
+/--
+info: ∀ {w : Nat} (a : BitVec w),
+  @LE.le (BitVec w) (@instLEBitVec w) a (BitVec.ofNat w (@OfNat.ofNat Nat 0 (instOfNatNat 0))) : Prop
+-/
+#guard_msgs in set_option pp.explicit true in
+#check ∀ {w : Nat} (a : BitVec w),  a  ≤ 0#w
+
+/--
+info: ∀ {w : Nat} (a : BitVec w),
+  @Eq Bool (@BitVec.slt w a (BitVec.ofNat w (@OfNat.ofNat Nat 0 (instOfNatNat 0)))) true : Prop
+-/
+#guard_msgs in set_option pp.explicit true in
+#check ∀ {w : Nat} (a : BitVec w),  a.slt 0#w
+
+
+def reflectAtomUnchecked (map : ReflectMap) (_w : Expr) (e : Expr) : MetaM ReflectResult := do
+  let (e, map) := map.findOrInsertExpr e
+  return { bvToIxMap := map, e := e }
+
+
+
+/--
+Return a new expression that this is **defeq** to, along with the expression of the environment that this needs.
+Crucially, when this succeeds, this will be in terms of `term`.
+and furthermore, it will reflect all terms as variables.
+
+Precondition: we assume that this is called on bitvectors.
+-/
+partial def reflectTermUnchecked (map : ReflectMap) (w : Expr) (e : Expr) : MetaM ReflectResult := do
+  -- TODO: bitvector contants.
+  match_expr e with
+  | BitVec.ofInt _wExpr iExpr =>
+    let i ← getIntValue? iExpr
+    match i with
+    | .some (-1) =>
+      let e := (mkConst ``Term.negOne)
+      return {bvToIxMap := map, e := e}
+    | _ => 
+      let (e, map) := map.findOrInsertExpr e
+      return { bvToIxMap := map, e := e }
+  | BitVec.ofNat _wExpr nExpr =>
+    let n ← getNatValue? nExpr
+    match n with
+    | .some 0 => 
+      let e := (mkConst ``Term.zero)
+      return {bvToIxMap := map, e := e}
+    | .some 1 =>
+      let e := (mkConst ``Term.one)
+      return {bvToIxMap := map, e := e}
+    | _ => 
+      let (e, map) := map.findOrInsertExpr e
+      return { bvToIxMap := map, e := e }
+  | HAnd.hAnd _bv _bv _bv _inst a b =>
+      let a ← reflectTermUnchecked map w a
+      let b ← reflectTermUnchecked a.bvToIxMap w b
+      let out := mkApp2 (mkConst ``Term.and) a.e b.e
+      return { b with e := out }
+  | HOr.hOr _bv _bv _bv _inst a b =>
+      let a ← reflectTermUnchecked map w a
+      let b ← reflectTermUnchecked a.bvToIxMap w b
+      let out := mkApp2 (mkConst ``Term.or) a.e b.e
+      return { b with e := out }
+  | HXor.hXor _bv _bv _bv _inst a b =>
+      let a ← reflectTermUnchecked map w a
+      let b ← reflectTermUnchecked a.bvToIxMap w b
+      let out := mkApp2 (mkConst ``Term.xor) a.e b.e
+      return { b with e := out }
+  | Complement.complement _bv _inst a =>
+      let a ← reflectTermUnchecked map w a
+      let out := mkApp (mkConst ``Term.not) a.e
+      return { a with e := out }
+  | HAdd.hAdd _bv _bv _bv _inst a b =>
+      let a ← reflectTermUnchecked map w a
+      let b ← reflectTermUnchecked a.bvToIxMap w b
+      let out := mkApp2 (mkConst ``Term.add) a.e b.e
+      return { b with e := out }
+  | HSub.hSub _bv _bv _bv _inst a b =>
+      let a ← reflectTermUnchecked map w a
+      let b ← reflectTermUnchecked a.bvToIxMap w b
+      let out := mkApp2 (mkConst ``Term.sub) a.e b.e
+      return { b with e := out }
+  | Neg.neg _bv _inst a =>
+      let a ← reflectTermUnchecked map w a
+      let out := mkApp (mkConst ``Term.neg) a.e
+      return { a with e := out }
+  -- incr
+  -- decr
+  | _ => 
+    let (e, map) := map.findOrInsertExpr e
+    return { bvToIxMap := map, e := e }
+
+set_option pp.explicit true in
+/--
+info: ∀ {w : Nat} (a b : BitVec w), Or (@Eq (BitVec w) a b) (And (@Ne (BitVec w) a b) (@Eq (BitVec w) a b)) : Prop
+-/
+#guard_msgs in 
+#check ∀ {w : Nat} (a b : BitVec w), a = b ∨ (a ≠ b) ∧ a = b
+
+/-- Return a new expression that this is defeq to, along with the expression of the environment that this needs, under which it will be defeq. -/
+partial def reflectPredicateAux (bvToIxMap : ReflectMap) (e : Expr) : MetaM ReflectResult := do
+  match_expr e with
+  | Eq α a b =>
+    match_expr α with 
+    | BitVec w => 
+      let a ←  reflectTermUnchecked bvToIxMap w a
+      let b ← reflectTermUnchecked a.bvToIxMap w b
+      return { bvToIxMap := b.bvToIxMap, e := mkAppN (mkConst ``Predicate.eq) #[a.e, b.e] }
+    | Bool =>
+      -- Sadly, recall that slt, sle are of type 'BitVec w → BitVec w → Bool',
+      -- so we get goal states of them form 'a <ₛb = true'.
+      -- So we need to match on 'Eq _ true' where '_' is 'slt'.
+      -- This makes me unhappy too, but c'est la vie.
+      let_expr true := b 
+        | throwError "only boolean conditionals allowed are 'bv.slt bv = true', 'bv.sle bv = true'. Found {indentD e}."
+      match_expr a with
+      | BitVec.slt w a b => 
+        let a ← reflectTermUnchecked bvToIxMap w a
+        let b ← reflectTermUnchecked a.bvToIxMap w b
+        return { bvToIxMap := b.bvToIxMap, e := mkAppN (mkConst ``Predicate.slt) #[a.e, b.e] }
+      | BitVec.sle w a b => 
+        let a ← reflectTermUnchecked bvToIxMap w a
+        let b ← reflectTermUnchecked a.bvToIxMap w b
+        return { bvToIxMap := b.bvToIxMap, e := mkAppN (mkConst ``Predicate.sle) #[a.e, b.e] }
+      | _ => 
+        throwError "unknown boolean conditional, expected 'bv.slt bv = true' or 'bv.sle bv = true'. Found {indentD e}"
+    | _ =>
+      throwError "unknown equality kind, expected 'bv = bv' or 'bv.slt bv = true' or 'bv.sle bv = true'. Found {indentD e}"
+  | Ne α a b =>
+    let_expr BitVec w := α | throwError "Expected typeclass to be BitVec w, found '{indentD α}' in {e} when matching against 'Ne'"
+    let a ← reflectTermUnchecked bvToIxMap w a
+    let b ← reflectTermUnchecked a.bvToIxMap w b
+    return { bvToIxMap := b.bvToIxMap, e := mkAppN (mkConst ``Predicate.neq) #[a.e, b.e] }
+  | LT.lt α _inst a b =>
+    let_expr BitVec w := α | throwError "Expected typeclass to be BitVec w, found '{indentD α}' in {indentD e} when matching against 'LT.lt'"
+    let a ← reflectTermUnchecked bvToIxMap w a
+    let b ← reflectTermUnchecked a.bvToIxMap w b
+    return { bvToIxMap := b.bvToIxMap, e := mkAppN (mkConst ``Predicate.ult) #[a.e, b.e] }
+  | LE.le α _inst a b =>
+    let_expr BitVec w := α | throwError "Expected typeclass to be BitVec w, found '{indentD α}' in {indentD e} when matching against 'LE.le'"
+    let a ← reflectTermUnchecked bvToIxMap w a
+    let b ← reflectTermUnchecked a.bvToIxMap w b
+    return { bvToIxMap := b.bvToIxMap, e := mkAppN (mkConst ``Predicate.ule) #[a.e, b.e] }
+  | Or p q =>
+    let p ← reflectPredicateAux bvToIxMap p
+    let q ← reflectPredicateAux p.bvToIxMap q
+    let out := mkApp2 (mkConst ``Predicate.lor) p.e q.e
+    return { q with e := out }
+  | And p q =>
+    let p ← reflectPredicateAux bvToIxMap p
+    let q ← reflectPredicateAux p.bvToIxMap q
+    let out := mkApp2 (mkConst ``Predicate.land) p.e q.e
+    return { q with e := out }
+  | _ => 
+     throwError "expected predicate over bitvectors (no quantification), found:  {indentD e}"
+
+/-- Name of the tactic -/
+def tacName : String := "bv_automata3"
+
+abbrev WidthToExprMap := Std.HashMap Expr Expr
+
+/--
+Find all bitwidths implicated in the given expression.
+Maps each length (the key) to an expression of that length.
+
+Find all bitwidths implicated in the given expression,
+by visiting subexpressions with visitExpr:
+    O(size of expr × inferType)
+-/
+def findExprBitwidths (target : Expr) : MetaM WidthToExprMap := do
+  let (_, out) ← StateT.run (go target) ∅
+  return out
+  where
+    go (target : Expr) : StateT WidthToExprMap MetaM Unit := do
+      -- Creates fvars when going inside binders.
+      forEachExpr target fun e => do
+        match_expr ← inferType e with
+        | BitVec n => 
+          -- TODO(@bollu): do we decide to normalize `n`? upto what?
+          modify (fun arr => arr.insert n.cleanupAnnotations e)
+        | _ => return ()
+
+/-- Return if expression 'e' is a bitvector of bitwidth 'w' -/
+private def Expr.isBitVecOfWidth (e : Expr) (w : Expr) : MetaM Bool := do
+  match_expr ← inferType e with
+  | BitVec w' => return w == w'
+  | _ => return false
+    
+
+/-- Revert all bitwidths of a given bitwidth and then run the continuation 'k'.
+This allows
+-/
+def revertBVsOfWidth (g : MVarId) (w : Expr) : MetaM MVarId := g.withContext do
+  let mut reverts : Array FVarId := #[]
+  for d in ← getLCtx do
+    if ← Expr.isBitVecOfWidth d.type w then
+      reverts := reverts.push d.fvarId
+  /- revert all the bitvectors of the given width in one fell swoop. -/
+  let (_fvars, g) ← g.revert reverts
+  return g
+  
+/-- generalize our mapping to get a single fvar -/
+def generalizeMap (g : MVarId) (e : Expr) : MetaM (FVarId × MVarId) :=  do
+  let (fvars, g) ← g.generalize #[{ expr := e : GeneralizeArg}]
+  --eNow target no longer depends on the particular bitvectors
+  if h : fvars.size = 1 then
+    return (fvars[0], g)
+  throwError"expected a single free variable from generalizing map {e}, found multiple..."
+
+#check reduceBool
+#check ofReduceBool
+
+/--
+Revert all hypotheses that have to do with bitvectors, so that we can use them.
+
+For now, we choose to revert all propositional hypotheses.
+The issue is as follows: Since our reflection fragment only deals with 
+goals in negation normal form, the naive algorithm would run an NNF pass
+and then try to reflect the hyp before reverting it. This is expensive and annoying to implement.
+
+Ideally, we would have a pass that quickly walks an expression to cheaply
+ee if it's in the BV fragment, and revert it if it is.
+For now, we use a sound overapproximation and revert everything.
+-/
+def revertBvHyps (g : MVarId) : MetaM MVarId := do
+  let (_, g) ← g.revert (← g.getNondepPropHyps)
+  return g
+
+/-- 
+Reflect an expression of the form:
+  ∀ ⟦(w : Nat)⟧ (← focus)
+  ∀ (b₁ b₂ ... bₙ : BitVec w),
+  <proposition about bitvectors>.
+
+Reflection code adapted from `elabNaticeDecideCoreUnsafe`,
+which explains how to create the correct auxiliary definition of the form
+`decideProprerty = true`, such that our goal state after using `ofReduceBool` becomes
+⊢ ofReduceBool decideProperty = true
+
+which is then indeed `rfl` equal to `true`. 
+-/
+def reflectUniversalWidthBVs (g : MVarId) : MetaM (List MVarId) := do
+  let ws ← findExprBitwidths (← g.getType)
+  let ws := ws.toArray
+  if h0: ws.size = 0 then throwError "found no bitvector in the target: {indentD (← g.getType)}"
+  else if hgt: ws.size > 1 then
+    let (w1, wExample1) := ws[0]
+    let (w2, wExample2) := ws[1]
+    let mExample := f!"{w1} → {wExample1}" ++ f!"{w2} → {wExample2}"
+    throwError "found multiple bitvector widths in the target: {indentD mExample}"
+  else
+    -- we have exactly one width
+    let (w, wExample) := ws[0]
+    if !w.isFVar then
+      throwError "expcted width to be a free variable, found with '{w}' (for bitvector '{wExample}')"
+    else
+      -- invariant: w is known to be an fvar.
+      let wFv := w.fvarId!
+      -- We can now revert hypotheses that are of this bitwidth.
+      let g ← revertBvHyps g
+          
+      -- Next, after reverting, we have a goal which we want to reflect.
+      -- we convert this goal to NNF
+      let .some g ← NNF.runNNFSimpSet g
+        | logInfo m!"simp automatically closed goal."
+          return[]
+      logInfo m!"goal after NNF: {indentD g}"
+      -- finally, we perform reflection.
+      let result ← reflectPredicateAux ∅ (← g.getType)
+      let bvToIxMapVal ← result.bvToIxMap.toExpr w
+      let target := (mkAppN (mkConst ``Predicate.denote) #[result.e, w, bvToIxMapVal])
+      let g ← g.replaceTargetDefEq target
+      logInfo m!"goal after reflection: {indentD g}"
+      let (mapFv, g) ← generalizeMap g bvToIxMapVal; 
+      let (_, g) ← g.revert #[mapFv]
+      -- Apply Predicate.denote_of_eval_eq.
+      let [g] ← g.apply <| (mkConst ``Predicate.denote_of_eval_eq) 
+        | throwError m!"Failed to apply `Predicate.denote_of_eval_eq` on goal '{indentD g}'"
+      let [g] ← g.apply <| (mkConst ``of_decide_eq_true) 
+        | throwError m!"Failed to apply `of_decide_eq_true on goal '{indentD g}'"
+      let [g] ← g.apply <| (mkConst ``Lean.ofReduceBool) 
+        | throwError m!"Failed to apply `of_decide_eq_true on goal '{indentD g}'"
+      return [g]
+
+/--
+Given a goal state of the form:
+  ∀ (w : Nat)
+  ∀ (b₁ b₂ ... bₙ : BitVec w),
+  <proposition about bitvectors>.
+
+decide the property by reduction to finite automata.
+
+TODO(@bollu): Also decide properties about finite widths, by extending to the maximal width and clearing the high bits?
+-/
+elab "bv_reflect" : tactic => do
+  liftMetaTactic fun g => do
+    reflectUniversalWidthBVs g
+
+
+elab "bv_automata3" : tactic => do
+  liftMetaTactic fun g => do
+    reflectUniversalWidthBVs g 
+
+  match ← getUnsolvedGoals  with
+  | [] => return ()
+  -- | TODO: replace with ofReduceBool
+  | [g] => do
+    logInfo m!"goal being decided: {indentD g}"
+    evalDecideCore `bv_automata3 (cfg := { native := true : Parser.Tactic.DecideConfig})
+  | _gs => throwError "expected single goal after reflecting, found multiple goals. quitting"
+  
+/-- Can solve explicitly quantified expressions with intros. bv_automata3. -/
+theorem eq1 : ∀ (w : Nat) (a : BitVec w), a = a := by
+  intros 
+  bv_automata3
+#print eq1
+
+/-- Can solve implicitly quantified expressions by directly invoking bv_automata3. -/
+theorem eq2 (w : Nat) (a : BitVec w) : a = a := by
+  bv_automata3
+#print eq1
+
+
+open NNF in
+
+example (w : Nat) (a b : BitVec w) : a + b = b + a := by
+  bv_automata3
+
+example (w : Nat) (a b : BitVec w) : (a + b = b + a) ∨ (a = 0#w) := by
+  bv_automata3
+
+example (w : Nat) (a b : BitVec w) : (a = 0#w) ∨ (a + b = b + a) := by
+  bv_automata3
+
+example (w : Nat) (a : BitVec w) : (a = 0#w) ∨ (a ≠ 0#w) := by
+  bv_automata3
+
+example (w : Nat) (a b : BitVec w) : (a + b = b + a) ∧ (a + 0#w = a) := by
+  bv_automata3
+
+example (w : Nat) (a b : BitVec w) : (a + 0#w = a) := by
+  bv_automata3
+
+example (w : Nat) (a b : BitVec w) : (a + b = b + a) ∧ (a + 0#w = a) := by
+  bv_automata3
+
+example (w : Nat) (a b : BitVec w) : (a ≠ b) → (b ≠ a) := by
+  bv_automata3
+
+/-- either a < b or b ≤ a -/
+example (w : Nat) (a b : BitVec w) : (a < b) ∨ (b ≤ a) := by
+  bv_automata3
+
+/-- Tricohotomy of < -/
+example (w : Nat) (a b : BitVec w) : (a < b) ∨ (b < a) ∨ (a = b) := by
+  bv_automata3
+
+/-- < implies not equals -/
+example (w : Nat) (a b : BitVec w) : (a < b) → (a ≠ b) := by
+  bv_automata3
+
+/-- <= and >= implies equals -/
+example (w : Nat) (a b : BitVec w) : ((a ≤ b) ∧ (b ≤ a)) → (a = b) := by
+  bv_automata3
+
+example (a b : BitVec 1) : (a - b).slt 0 → a.slt b := by
+  fail_if_success bv_decide
+  -- The prover found a counterexample, consider the following assignment:
+  -- a = 0x0#1
+  -- b = 0x1#1
+  sorry
+
+/-- Tricohotomy of slt. Currently fails! -/
+example (w : Nat) (a b : BitVec w) : (1#w = 0#w) ∨ ((a - b).slt 0 → a.slt b) := by
+  bv_automata3
+
+
+/-- Tricohotomy of slt. Currently fails! -/
+example (w : Nat) (a b : BitVec w) : (a.slt b) ∨ (b.sle a) := by
+  bv_automata3
+  -- TODO: I don't understand this metaprogramming error, I must be building the term weirdly...
+
+/-- Tricohotomy of slt. Currently fails! -/
+example (w : Nat) (a b : BitVec w) : (a.slt b) ∨ (b.slt a) ∨ (a = b) := by
+  bv_automata3
+  -- TODO: I don't understand this metaprogramming error, I must be building the term weirdly...
+
+/-- a <=s b and b <=s a implies a = b-/
+example (w : Nat) (a b : BitVec w) : ((a.sle b) ∧ (b.sle a)) → a = b := by
+  bv_automata3
+  -- TODO: I don't understand this metaprogramming error, I must be building the term weirdly...
+
+/-- In bitwidth 0, all values are equal.
+In bitwidth 1, 1 + 1 = 0.
+In bitwidth 2, 1 + 1 = 2 ≠ 0#2
+For all bitwidths ≥ 2, we know that a ≠ a + 1
+-/
+example (w : Nat) (a : BitVec w) : (a ≠ a + 1#w) ∨ (1#w + 1#w = 0#w) ∨ (1#w = 0#w):= by
+  bv_automata3
+
+/-- If we have that 'a &&& a = 0`, then we know that `a = 0` -/
+example (w : Nat) (a : BitVec w) : (a &&& a = 0#w) → a = 0#w := by
+  bv_automata3
+
+/-
+Is this true at bitwidth 1? Not it is not!
+So we need an extra hypothesis that rules out bitwifth 1.
+We do this by saying that either the given condition, or 1+1 = 0.
+I'm actually not sure why I need to rule out bitwidth 0? Mysterious!
+-/
+example (w : Nat) (a : BitVec w) : (1#w = 0#w) ∨ (1#w + 1#w = 0#w) ∨ ((a = - a) → a = 0#w) := by
+  bv_automata3
+
+
+/-
+We can say that we are at bitwidth 1 by saying that 1 + 1 = 0.
+When we have this, we then explicitly enumerate the different values that a can have.
+Note that this is pretty expensive.
+-/
+example (w : Nat) (a : BitVec w) : (1#w + 1#w = 0#w) → (a = 0#w ∨ a = 1#w) := by
+  bv_automata3
+
+
+
+example (w : Nat) (a b : BitVec w) : (a + b = 0#w) → a = - b := by
+  bv_automata3
+
+
+/-- Can use implications -/
+theorem eq3 (w : Nat) (a b : BitVec w) : (a &&& b = 0#w) → ((a + b) = (a ||| b)) := by
+  bv_nnf
+  bv_automata3
+
+#print eq3
+
+
+open NNF in
+/-- Can exploit hyps -/
+theorem eq4 (w : Nat) (a b : BitVec w) (h : a &&& b = 0#w) : a + b = a ||| b := by
+  bv_automata3
+
+#print eq3
+
+/-- error: expcted width to be a free variable, found with '10' (for bitvector 'b') -/
+#guard_msgs in example : ∀ (a b : BitVec 10), a = b := by
+  intros a b
+  bv_reflect
+
+
+section BvAutomataTests
+
+/-!
+# Test Cases
+-/
+
+def alive_1 {w : ℕ} (x x_1 x_2 : BitVec w) : (x_2 &&& x_1 ^^^ x_1) + 1#w + x = x - (x_2 ||| ~~~x_1) := by
+  bv_automata3
+
+/--
+info: 'Reflect.alive_1' depends on axioms: [propext,
+ sorryAx,
+ Classical.choice,
+ Lean.ofReduceBool,
+ Lean.trustCompiler,
+ Quot.sound]
+-/
+#guard_msgs in #print axioms alive_1
+
+def false_statement {w : ℕ} (x y : BitVec w) : x = y := by
+  fail_if_success bv_automata3
+  sorry
+
+def test_OfNat_ofNat (x : BitVec 1) : 1#1 + x = x + 1#1 := by
+  fail_if_success bv_automata3 -- can't decide things for fixed bitwidth.
+  sorry
+
+
+
+def test0 {w : Nat} (x y : BitVec w) : x + 0#w = x := by
+  bv_automata3
+
+
+def test_simple2 {w : Nat} (x y : BitVec w) : x = x := by
+  bv_automata3
+
+def test1 {w : Nat} (x y : BitVec w) : (x ||| y) - (x ^^^ y) = x &&& y := by
+  bv_automata3
+
+
+def test4 (x y : BitVec w) : (x + -y) = (x - y) := by
+  bv_automata3
+
+def test5 (x y z : BitVec w) : (x + y + z) = (z + y + x) := by
+  bv_automata3
+
+
+def test6 (x y z : BitVec w) : (x + (y + z)) = (x + y + z) := by
+  bv_automata3
+
+def test11 (x y : BitVec w) : (x + y) = ((x |||  y) +  (x &&&  y)) := by
+  bv_automata3
+
+
+def test15 (x y : BitVec w) : (x - y) = (( x &&& (~~~ y)) - ((~~~ x) &&&  y)) := by
+  bv_automata3
+
+
+def test17 (x y : BitVec w) : (x ^^^ y) = ((x ||| y) - (x &&& y)) := by
+  bv_automata3
+
+
+def test18 (x y : BitVec w) : (x &&&  (~~~ y)) = ((x ||| y) - y) := by
+  bv_automata3
+
+
+def test19 (x y : BitVec w) : (x &&&  (~~~ y)) = (x -  (x &&& y)) := by
+  bv_automata3
+
+
+def test21 (x y : BitVec w) : (~~~(x - y)) = (~~~x + y) := by
+  bv_automata3
+
+def test23 (x y : BitVec w) : (~~~(x ^^^ y)) = ((x &&& y) + ~~~(x ||| y)) := by
+  bv_automata3
+
+def test24 (x y : BitVec w) : (x ||| y) = (( x &&& (~~~y)) + y) := by
+  bv_automata3
+
+def test25 (x y : BitVec w) : (x &&& y) = (((~~~x) ||| y) - ~~~x) := by
+  bv_automata3
+
+def test26 {w : Nat} (x y : BitVec w) : 1#w + x + 0#w = 1#w + x := by
+  bv_automata3
+
+/-- NOTE: this fails since we don't support literals yet! -/
+def test27 (x y : BitVec w) : 2#w + x  = 1#w  + x + 1#w := by
+  fail_if_success bv_automata3
+  sorry
+
+def test28 {w : Nat} (x y : BitVec w) : x &&& x &&& x &&& x &&& x &&& x = x := by
+  bv_automata3
+
+end BvAutomataTests
+
+end Reflect
+
