SSA/Projects/InstCombine/ForStd.lean
@@ -5,15 +5,15 @@ Released under Apache 2.0 license as described in the file LICENSE.
 namespace BitVec
 
 
-notation:50 x " ≤ᵤ " y => BitVec.ule x y
-notation:50 x " <ᵤ " y => BitVec.ult x y
 notation:50 x " ≥ᵤ " y => BitVec.ule y x
 notation:50 x " >ᵤ " y => BitVec.ult y x
+notation:50 x " ≤ᵤ " y => BitVec.ule x y
+notation:50 x " <ᵤ " y => BitVec.ult x y
 
-notation:50 x " ≤ₛ " y => BitVec.sle x y
-notation:50 x " <ₛ " y => BitVec.slt x y
 notation:50 x " ≥ₛ " y => BitVec.sle y x
 notation:50 x " >ₛ " y => BitVec.slt y x
+notation:50 x " ≤ₛ " y => BitVec.sle x y
+notation:50 x " <ₛ " y => BitVec.slt x y
 
 instance {n} : ShiftLeft (BitVec n) := ⟨fun x y => x <<< y.toNat⟩
 
